---
title: "Derivatives"
format: html
toc: false
---
 
__Contant Rule__: Taking the derivative of a constant is $0$

$$
f(x) = c
$$
$$
f'(x) = 0
$$

----

__Power Rule__: 
$$
f(x) = x^{n}
$$
$$
f'(x) = nx^{n-1}
$$

----

__Sum & Difference Rules__: Taking the derivative of the sum or difference of $g(x)$ and $f(x)$ is the same as the derivative of $g(x)$ plus or minus the derivative of $f(x)$
$$
\frac{\text{d}}{\text{dx}}(f(x) \pm g(x)) 
\text{ } = \text{ } 
\frac{\text{d}}{\text{dx}}(f(x)) \pm \frac{\text{d}}{\text{dx}}(g(x))
$$

----

__Constant Multiple Rules__: Taking the derivative of a constant times a derivative is the same as the constant multiplied by the derivative
$$
\frac{\text{d}}{\text{dx}}(kf(x)) 
\text{ } = \text{ } 
k\frac{\text{d}}{\text{dx}}(f(x))
$$

<details>
<summary>Example</summary>

$$
\frac{\text{d}}{\text{dx}}\left(\frac{3x}{2}\right)
\text{ } \rightarrow \text{ }
\frac{3}{2}\frac{\text{d}}{\text{dx}}\left(x\right)
\text{ } \rightarrow \text{ }
\frac{3}{2}\left(x^{1-1}\right)
\text{ } \rightarrow \text{ }
\frac{3}{2}
$$

</details>

---- 

__Product Rule__: Taking the derivative of a function times a function
$$
\frac{\text{d}}{\text{dx}}(f(x)g(x)) 
\text{ } = \text{ } 
f'(x)g(x) + g'(x)f(x)
$$

----

__Quotient Rule__: Taking the derivative of a function divided by a function
$$
\frac{\text{d}}{\text{dx}} \left(\frac{f(x)}{g(x)}\right) 
\text{ } = \text{ } 
\frac{f'(x)g(x)-g'(x)f(x)}{(g(x))^{2}}
$$

24+2 x (-25+6 x (2+x)) 

----

__Chain Rule__: to allow us to differentiate composite funtions

$$h(x) = (f \circ g)(x) = f(g(x))$$
$$h'(x) = f'(g(x))g'(x)$$

----

__Chain and Power Rules Combined__:
$$
h(x) = (g(x))^{n}
$$
$$
h'(x) = n(g(x))^{n-1}g'(x)
$$

<details>
<summary>Example</summary>

$$
\textbf{Find }\frac{\text{dy}}{\text{dx}} \text{ if } y = (2-x^{2})^{-5}
$$
$$
\textbf{Answer: } -5(2-x^{2})^{-6}(-2x)
$$

</details>


<br>

:::{.callout-tip collapse="true"}
# Product and Quotient Rules Practice 1

These problems...

![](deriv_graph_problem.png)

They say $h(x) = f(x)*g(x)$

They want us to find $h'(x)$

The *product rule* applies here because two functions are being multiplied together 

The tricky part is to remember how to find $f(x)$, $f'(x)$, $g(x)$, and $g'(x)$

To find functions, just plug in the $X$ and there there's the $Y$. 

The derivatives of functions are the slope at that point. Here we see that the slope of $f(x)$ at 5 is $2$ and the slope of $g(x)$ at 5 is $1$


<br>

:::


<br></br>

## Common Errors/Notes

- Remember that the denominator of the quotient rule is $(g(x))^{2}$, not $(g'(x))^{2}$


## Other Examples: 

<details>
<summary>Example</summary>

Find $k'(x)$
$$
k(x) = -2x\left(h(x) + 2x^{2}g(x))\right)
$$
From here, distribute the $-2x$
$$
k(x) = -2x\left(h(x) + 2x^{2}g(x))\right)
$$
Now take the derivative of each side
$$
\frac{\text{d}}{\text{dx}} \left(k(x)\right) 
\text{ } = \text{ } 
\frac{\text{d}}{\text{dx}} \left( -2x\left(h(x) + 2x^{2}g(x))\right) \right)
$$
Notice the double chain rule
$$
\frac{\text{d}}{\text{dx}} \left(k(x)\right) 
\text{ } = \text{ } 
\frac{\text{d}}{\text{dx}} \left(-2x * h(x) \right) + \frac{\text{d}}{\text{dx}} \left(-4x^{3} * g(x) \right)
$$
Derivative on the right
$$
\frac{\text{d}}{\text{dx}} \left(-2x * h(x) \right) 
\rightarrow 
-2*h(x) - 2x * h'(x)
$$
Derivative on the left
$$
\frac{\text{d}}{\text{dx}} \left(-4x^{3} * g(x) \right) 
\rightarrow 
-12x^{2} * g(x) - 4x^{3} * g'(x)
$$
Now combine everything
$$
k'(x) = \left(-2*h(x) - 2x * h'(x)\right) + \left(-12x^{2} * g(x) - 4x^{3} * g'(x)\right)
$$
Now substitute the values given and use algebra to simplify it

</details>

<br><br>


## Second Derivative Section

This is about: 
- taking the derivative a second time
- local maximun and minimum
- first and second derivative tests

- decreasing in polynomial each time a derivative is taken






<br><br>


<!-- <iframe src="quarto.org" title="W3Schools Free Online Web Tutorials" width="100%" height="300" style="border:1px solid black;"></iframe> -->







d/dx == d*f(x)/dx
Find the derivative of f(x) in terms of x 





<br>



# Advanced Algebra Syntax


$$
\log_{}{x} 
=
\log_{10}{x}
$$

$$
\ln{x} 
= 
\log_{e}{x}
$$

$$
e = 2.718\text{...}
$$




----

# Notes from Hawanay's Dec 2nd Tutoring Appointment

## 1) Logarithms

$$
b^{e} = n \text{ is the same as } \log_{b}n = e
$$

$$
\log(x) = \log_{10}(x)
$$
$$
\log_{e}(x) = \ln(x) 
$$

## 2) Derivative of $e$ & $e^{u}$

Derivative of $e^{x} = e^{x}$

- This is because the derivative of the function is the function

Derivative of $e^{u} = e^{u}u'$

:::{.callout-tip appearance="minimal"}
# Example:
$$
e^{x^{2}} = 2e^{x^{2}}
$$
:::


## 3) Derivative of a Natural Log 

$$
\frac{d}{dx}(\ln x) = \frac{x'}{x}
$$

Or... is it $\frac{d}{dx}(\ln x) = \frac{1}{x}$? I learned the method above in tutoring and on the tutoring center's math sheet, but I see on Knewton that the other fraction is used. 


Apparently there is a way to do this using the chain rule, but she does not reccomend that method, but rather this rule. 

## 4) Order of Operations

$-1(x+5)^{-2}$, the correct order of PEMDAS is to do the $-2$ exponent first, the the multiplication of $-1$ times the base. 

Think of it like this, $-1 * (x+5)^{-2}$

P
**E**
**M**
D
A
S


Exponents come before multiplication


## 5) See when to use the Chain Rule

Taking that problem above a step to the side, 

The derivative of $-1(x+5)^{-2}$ is 

$$

$$

## 6?

When given $k(x) = x\left(2x+\frac{1}{x+3}\right)$ to find $k'(x)$, there are two ways. Either: 

- preform the product rule from here 

or 

- distribute the $x$, then take the derivative from there (which will include either a quotient rule or a chain & product rule)

---- 

## Chain Rule Examples

:::{.callout-tip appearance="minimal"}
# Example:

$h(x) = 4\sin^{11}(x)$, find $h'(x)$

This one confused me. I guess it is a chain rule. Here's my work:

$h(x) = 4\sin^{11}(x) \rightarrow 4(\sin(x))^{11}$

- $f(x) = 4(\sin(x))^{11}$

- $f'(x) = 44(u)^{10} \rightarrow 44(\sin(x))^{10}$

- $g(x) = \sin(x)$

- $g'(x) = \cos(x)$

Formula: $h'(x) = f'(g(x)) * g'(x)$

$h'(x) = 44(\sin(x))^{10} * \cos(x)$

I think the $4$ is getting in my way of seeing that $\sin^{11}(x)$ is a chain rule. We treat the $4$ with the *constant multiple rule*. $\sin^{11}(x)$ can be better seen as a chain rule when written as $(\sin(x))^{11}$. $\sin(x) = u$; $(\sin(x))^{11} = u^{11}$
:::